coq/NNRC/Typing/TNNRCEq.v
@@ -15,7 +15,6 @@
  *)
 
 Section TNNRCEq.
-
   Require Import Equivalence.
   Require Import Morphisms.
   Require Import Setoid.
@@ -24,25 +23,29 @@ Section TNNRCEq.
   Require Import String.
   Require Import List.
   Require Import Arith.
+  Require Import BasicSystem.
+  Require Import cNNRCSystem.
+  Require Import NNRC.
+  Require Import NNRCEq.
+  Require Import TNNRC.
 
-  Require Import Utils BasicSystem.
-  Require Import cNNRC NNRC TNNRC.
-
-  (* Named Nested Relational Calculus *)
-
-  (* A different kind of equivalence for rewrites *)
+  (* A type-safe equivalence for rewrites *)
 
   Context {m:basic_model}.
 
   Definition tnnrc_ext_rewrites_to (e1 e2:nnrc) : Prop :=
-    forall (τenv : tbindings) (τout:rtype),
-      nnrc_ext_type τenv e1 τout ->
-      (nnrc_ext_type τenv e2 τout) /\ (forall (env:bindings),
-                                     bindings_type env τenv -> @nnrc_ext_eval _ brand_relation_brands env e1 = @nnrc_ext_eval _ brand_relation_brands env e2).
+    forall (τcenv τenv : tbindings) (τout:rtype),
+      nnrc_ext_type τcenv τenv e1 τout ->
+      (nnrc_ext_type τcenv τenv e2 τout)
+      /\ (forall (cenv:bindings),
+          forall (env:bindings),
+             bindings_type cenv τcenv ->
+             bindings_type env τenv ->
+             @nnrc_ext_eval _ brand_relation_brands cenv env e1
+             = @nnrc_ext_eval _ brand_relation_brands cenv env e2).
 
   Notation "e1 ⇒ᶜ e2" := (tnnrc_ext_rewrites_to e1 e2) (at level 80).
 
-  Require Import NNRCEq.
   Open Scope nnrc_scope.
 
   Lemma data_normalized_bindings_type_map env τenv :
@@ -57,7 +60,9 @@ Section TNNRCEq.
   
   Lemma nnrc_ext_rewrites_typed_with_untyped (e1 e2:nnrc) :
     e1 ≡ᶜ e2 ->
-    (forall  {τenv: tbindings} {τout:rtype}, nnrc_ext_type τenv e1 τout -> nnrc_ext_type τenv e2 τout)
+    (forall {τcenv: tbindings}
+            {τenv: tbindings}
+            {τout:rtype}, nnrc_ext_type τcenv τenv e1 τout -> nnrc_ext_type τcenv τenv e2 τout)
     -> e1 ⇒ᶜ e2.
   Proof.
     intros.
@@ -70,14 +75,10 @@ Section TNNRCEq.
    * Proper stuff *
    ****************)
 
-  Require Import TcNNRC TOps.
-  
   Hint Constructors nnrc_type.
   Hint Constructors unaryOp_type.
   Hint Constructors binOp_type.
 
-  Require Import ROpsEq.
-  
   Global Instance tnnrc_ext_rewrites_to_pre : PreOrder tnnrc_ext_rewrites_to.
   Proof.
     constructor; red; intros.
@@ -85,16 +86,27 @@ Section TNNRCEq.
       split; try assumption; intros.
       reflexivity.
     - unfold tnnrc_ext_rewrites_to in *; intros.
-      specialize (H τenv τout H1).
+      specialize (H τcenv τenv τout H1).
       elim H; clear H; intros.
-      specialize (H0 τenv τout H).
+      specialize (H0 τcenv τenv τout H).
       elim H0; clear H0; intros.
       split; try assumption; intros.
-      rewrite (H2 env); try assumption.
-      rewrite (H3 env); try assumption.
+      rewrite (H2 cenv env); try assumption.
+      rewrite (H3 cenv env); try assumption.
       reflexivity.
   Qed.
   
+  (* NNRCGetConstant *)
+
+  Global Instance nnrc_ext_get_constant_tproper:
+    Proper (eq ==> tnnrc_ext_rewrites_to) NNRCGetConstant.
+  Proof.
+    unfold Proper, respectful, tnnrc_ext_rewrites_to; intros.
+    rewrite <- H.
+    split; try assumption.
+    intros; reflexivity.
+  Qed.
+
   (* NNRCVar *)
 
   Global Instance nnrc_ext_var_tproper:
@@ -128,15 +140,15 @@ Section TNNRCEq.
     rewrite H in *; clear H.
     inversion H2; clear H2; subst.
     econstructor; eauto.
-    specialize (H0  τenv τ₁ H8); elim H0; clear H0 H8; intros.
-    specialize (H1  τenv τ₂ H9); elim H1; clear H1 H9; intros.
+    specialize (H0 τcenv τenv τ₁ H8); elim H0; clear H0 H8; intros.
+    specialize (H1 τcenv τenv τ₂ H9); elim H1; clear H1 H9; intros.
     econstructor; eauto; intros.
     intros.
-    specialize (H0  τenv τ₁ H8); elim H0; clear H0 H8; intros.
-    specialize (H1  τenv τ₂ H9); elim H1; clear H1 H9; intros.
+    specialize (H0 τcenv τenv τ₁ H8); elim H0; clear H0 H8; intros.
+    specialize (H1 τcenv τenv τ₂ H9); elim H1; clear H1 H9; intros.
     unfold nnrc_ext_eval in *.
     simpl.
-    rewrite (H2 env H); rewrite (H3 env H); reflexivity.
+    rewrite (H3 cenv env H H2); rewrite (H4 cenv env H H2); reflexivity.
   Qed.
   
   (* NNRCUnop *)
@@ -149,11 +161,11 @@ Section TNNRCEq.
     inversion H1; clear H1; subst.
     econstructor; eauto.
     econstructor; eauto.
-    specialize (H0  τenv τ₁ H6); elim H0; clear H0 H6; intros; assumption.
+    specialize (H0 τcenv τenv τ₁ H6); elim H0; clear H0 H6; intros; assumption.
     intros.
-    specialize (H0  τenv τ₁ H6); elim H0; clear H0 H6; intros.
+    specialize (H0 τcenv τenv τ₁ H6); elim H0; clear H0 H6; intros.
     unfold nnrc_ext_eval in *.
-    simpl. rewrite (H1 env H); reflexivity.
+    simpl. rewrite (H2 cenv env H H1); reflexivity.
   Qed.
 
   (* NNRCLet *)
@@ -164,48 +176,47 @@ Section TNNRCEq.
     unfold Proper, respectful, tnnrc_ext_rewrites_to; intros.
     unfold nnrc_ext_eval,nnrc_ext_type in *.
     inversion H2; clear H2; subst.
-    specialize (H0 τenv τ₁ H8); elim H0; clear H0 H8; intros.
-    specialize (H1 ((y, τ₁) :: τenv) τout H9); elim H1; clear H1 H9; intros.
+    specialize (H0 τcenv τenv τ₁ H8); elim H0; clear H0 H8; intros.
+    specialize (H1 τcenv ((y, τ₁) :: τenv) τout H9); elim H1; clear H1 H9; intros.
     econstructor; eauto.
     econstructor; eauto.
     intros; simpl.
-    rewrite (H0 env H3).
-    case_eq (nnrc_core_eval brand_relation_brands env (nnrc_ext_to_nnrc y0));
+    rewrite (H0 cenv env H3 H4).
+    case_eq (nnrc_core_eval brand_relation_brands cenv env (nnrc_ext_to_nnrc y0));
       intros; try reflexivity.
-    rewrite (H2 ((y, d) :: env)); try reflexivity.
+    rewrite (H2 cenv ((y, d) :: env) H3); try reflexivity.
     unfold bindings_type.
     apply Forall2_cons; try assumption.
     simpl; split; try reflexivity.
-    generalize (@typed_nnrc_ext_yields_typed_data _ τ₁ env τenv y0 H3 H); intros.
-    elim H5; intros.
-    elim H6; clear H6; intros.
+    generalize (@typed_nnrc_ext_yields_typed_data _ τcenv τ₁ cenv env τenv y0 H3 H4 H); intros.
+    elim H6; intros.
+    elim H7; clear H7; intros.
     unfold nnrc_ext_eval,nnrc_ext_type in *.
-    rewrite H4 in H6.
-    inversion H6; assumption.
+    rewrite H5 in H7.
+    inversion H7; assumption.
   Qed.
     
   (* NNRCFor *)
 
-  Require Import TData.
-  
-  Lemma dcoll_wt (l:list data) (τ:rtype) (τenv:tbindings) (env:bindings) (e:nnrc):
+  Lemma dcoll_wt (l:list data) (τ:rtype) (τcenv τenv:tbindings) (cenv env:bindings) (e:nnrc):
+    bindings_type cenv τcenv ->
     bindings_type env τenv ->
-    nnrc_type τenv e (Coll τ) ->
-    nnrc_core_eval brand_relation_brands env e = Some (dcoll l) ->
+    nnrc_type τcenv τenv e (Coll τ) ->
+    nnrc_core_eval brand_relation_brands cenv env e = Some (dcoll l) ->
     forall x:data, In x l -> (data_type x τ).
   Proof.
     intros.
-    generalize (@typed_nnrc_yields_typed_data _ (Coll τ) env τenv e H H0); intros.
-    elim H3; clear H3; intros.
-    elim H3; clear H3; intros.
-    rewrite H3 in H1.
-    inversion H1; clear H1.
+    generalize (@typed_nnrc_yields_typed_data _ τcenv (Coll τ) cenv env τenv e H H0 H1); intros.
+    elim H4; clear H4; intros.
+    elim H4; clear H4; intros.
+    rewrite H4 in H2.
+    inversion H2; clear H2.
     subst.
-    dependent induction H4.
+    dependent induction H5.
     rtype_equalizer.
     subst.
-    rewrite Forall_forall in H1.
-    apply (H1 x0 H2).
+    rewrite Forall_forall in H2.
+    apply (H2 x0 H3).
   Qed.
 
   Global Instance nnrc_ext_for_tproper :
@@ -213,34 +224,34 @@ Section TNNRCEq.
   Proof.
     unfold Proper, respectful, tnnrc_ext_rewrites_to; intros.
     inversion H2; clear H2; subst.
-    specialize (H0  τenv (Coll τ₁) H8); elim H0; clear H0 H8; intros.
-    specialize (H1  ((y, τ₁) :: τenv) τ₂ H9); elim H1; clear H1 H9; intros.
+    specialize (H0 τcenv τenv (Coll τ₁) H8); elim H0; clear H0 H8; intros.
+    specialize (H1 τcenv ((y, τ₁) :: τenv) τ₂ H9); elim H1; clear H1 H9; intros.
     econstructor; eauto.
     econstructor; eauto.
     intros; simpl.
     unfold nnrc_ext_eval,nnrc_ext_type in *; simpl.
-    rewrite (H0 env H3).
-    case_eq (nnrc_core_eval brand_relation_brands env (nnrc_ext_to_nnrc y0));
+    rewrite (H0 cenv env H3 H4).
+    case_eq (nnrc_core_eval brand_relation_brands cenv env (nnrc_ext_to_nnrc y0));
       intros; try reflexivity.
     destruct d; try reflexivity.
     assert (forall x, In x l -> (data_type x τ₁))
       by
-        (apply (dcoll_wt l τ₁ τenv env (nnrc_ext_to_nnrc y0)); assumption).
-    clear H4 H.
+        (apply (dcoll_wt l τ₁ τcenv τenv cenv env (nnrc_ext_to_nnrc y0)); assumption).
+    clear H5 H.
     induction l; try reflexivity.
     simpl in *.
     assert (forall x : data, In x l -> data_type x τ₁)
-      by (intros; apply (H5 x); right; assumption).
+      by (intros; apply (H6 x); right; assumption).
     specialize (IHl H); clear H.
-    rewrite (H2 ((y, a) :: env)).
-    destruct (nnrc_core_eval brand_relation_brands ((y, a) :: env) (nnrc_ext_to_nnrc y1)); try reflexivity.
-    - destruct ((rmap (fun d1 : data => nnrc_core_eval brand_relation_brands ((y, d1) :: env) (nnrc_ext_to_nnrc x1)) l));
-      destruct ((rmap (fun d1 : data => nnrc_core_eval brand_relation_brands ((y, d1) :: env) (nnrc_ext_to_nnrc y1)) l));
+    rewrite (H2 cenv ((y, a) :: env) H3).
+    destruct (nnrc_core_eval brand_relation_brands cenv ((y, a) :: env) (nnrc_ext_to_nnrc y1)); try reflexivity.
+    - destruct ((rmap (fun d1 : data => nnrc_core_eval brand_relation_brands cenv ((y, d1) :: env) (nnrc_ext_to_nnrc x1)) l));
+      destruct ((rmap (fun d1 : data => nnrc_core_eval brand_relation_brands cenv ((y, d1) :: env) (nnrc_ext_to_nnrc y1)) l));
       simpl in *; try congruence.
     - unfold bindings_type.
       apply Forall2_cons; try assumption.
       simpl; split; try reflexivity.
-      apply (H5 a); left; reflexivity.
+      apply (H6 a); left; reflexivity.
   Qed.
     
   (* NNRCIf *)
@@ -252,14 +263,14 @@ Section TNNRCEq.
   Proof.
     unfold Proper, respectful, tnnrc_ext_rewrites_to; intros.
     inversion H2; clear H2; subst.
-    specialize (H  τenv Bool H7); elim H; clear H H7; intros.
-    specialize (H0  τenv τout H9); elim H0; clear H0 H9; intros.
-    specialize (H1  τenv τout H10); elim H1; clear H1 H10; intros.
+    specialize (H τcenv τenv Bool H7); elim H; clear H H7; intros.
+    specialize (H0 τcenv τenv τout H9); elim H0; clear H0 H9; intros.
+    specialize (H1 τcenv τenv τout H10); elim H1; clear H1 H10; intros.
     econstructor; eauto.
     econstructor; eauto.
     intros; simpl.
     unfold nnrc_ext_eval,nnrc_ext_type in *; simpl.
-    rewrite (H2 env H5). rewrite (H3 env H5). rewrite (H4 env H5).
+    rewrite (H2 cenv env H5 H6). rewrite (H3 cenv env H5 H6). rewrite (H4 cenv env H5 H6).
     reflexivity.
   Qed.
 
@@ -275,19 +286,19 @@ Section TNNRCEq.
     subst.
     simpl in H4.
     inversion H4; clear H4; subst.
-    destruct (H _ _ H10).
-    destruct (H1 _ _ H11).
-    destruct (H3 _ _ H12).
+    destruct (H _ _ _ H10).
+    destruct (H1 _ _ _ H11).
+    destruct (H3 _ _ _ H12).
     clear H H1 H3.
     simpl.
     split; [eauto | ]; intros.
     rewrite H2; trivial.
-    destruct (@typed_nnrc_yields_typed_data _ _ _ _ _  H H0) as [?[??]].
-    rewrite H1.
-    apply data_type_Either_inv in H3.
-    destruct H3 as [[?[??]]|[?[??]]]; subst.
-    - apply H5. constructor; simpl; intuition; eauto.
-    - eapply H7. constructor; simpl; intuition; eauto.
+    destruct (@typed_nnrc_yields_typed_data _ _ _ _ _ _ _ H H1 H0) as [?[??]].
+    rewrite H3.
+    apply data_type_Either_inv in H8.
+    destruct H8 as [[?[??]]|[?[??]]]; subst.
+    - apply (H5 _ _ H). constructor; simpl; intuition; eauto.
+    - eapply (H7 _ _ H). constructor; simpl; intuition; eauto.
   Qed.
 
   (* NNRCGroupBy *)
@@ -323,6 +334,6 @@ Notation "e1 ⇒ᶜ e2" := (tnnrc_ext_rewrites_to e1 e2) (at level 80).
 
 (* 
 *** Local Variables: ***
-*** coq-load-path: (("../../../coq" "QCert")) ***
+*** coq-load-path: (("../../../coq" "Qcert")) ***
 *** End: ***
 *)
