coq/Compiler/QLib/QUtil.v
@@ -39,8 +39,8 @@ Module QUtil(runtime:CompilerRuntime).
   (* Processing for input or output of queries *)
   Definition validate_lifted_success := validate_lifted_success.
 
-  Definition mkDistLoc := mkConstants mkDistLoc. (* XXX Where should mkConstants be? *)
-  Definition mkDistWorld env := mkConstants (mkDistWorld env). (* XXX Where should mkConstants be? *)
+  Definition mkDistLoc := mkDistLoc.
+  Definition mkDistWorld env := mkDistWorld env.
 End QUtil.
 
 (*
