coq/cNNRC/Lang/cNNRCNorm.v
@@ -14,92 +14,89 @@
  * limitations under the License.
  *)
 
-Section cNNRCProp.
-
+Section cNNRCNorm.
   Require Import String.
   Require Import List.
   Require Import Arith.
   Require Import EquivDec.
   Require Import Morphisms.
-
-  Require Import Utils BasicRuntime.
-
+  Require Import BasicRuntime.
   Require Import cNNRC.
 
   (** Named Nested Relational Calculus *)
 
   Context {fruntime:foreign_runtime}. 
   Context (h:brand_relation_t).
+  Context (c:bindings).
  
   (* evaluation preserves normalization *)
   Lemma nnrc_core_eval_normalized env e {o} :
-    nnrc_core_eval h env e = Some o ->
+    Forall (data_normalized h) (map snd c) ->
+    nnrc_core_eval h c env e = Some o ->
     Forall (data_normalized h) (map snd env) ->
     data_normalized h o.
   Proof.
-    revert env o. nnrc_cases (induction e) Case.
+    revert env o. nnrc_cases (induction e) Case; simpl; intros env o Hc; intros.
+    - Case "NNRCGetConstant"%string.
+      rewrite Forall_forall in Hc.
+      unfold edot in H. apply assoc_lookupr_in in H.
+      apply (Hc o).
+      rewrite in_map_iff.
+      exists (v,o); eauto.
     - Case "NNRCVar"%string.
-      simpl; intros.
       rewrite Forall_forall in H0.
       apply lookup_in in H.
       apply (H0 o).
       rewrite in_map_iff.
       exists (v,o); eauto.
     - Case "NNRCConst"%string.
-      simpl; intros.
       inversion H; subst; intros.
       apply normalize_normalizes.
     - Case "NNRCBinop"%string.
-      simpl; intros.
-      case_eq (nnrc_core_eval h env e1); [intros ? eqq1 | intros eqq1];
+      case_eq (nnrc_core_eval h c env e1); [intros ? eqq1 | intros eqq1];
       (rewrite eqq1 in *;
-      case_eq (nnrc_core_eval h env e2); [intros ? eqq2 | intros eqq2];
+      case_eq (nnrc_core_eval h c env e2); [intros ? eqq2 | intros eqq2];
       rewrite eqq2 in *); simpl in *; try discriminate.
       eapply fun_of_binop_normalized; eauto.
     - Case "NNRCUnop"%string.
-      simpl; intros.
-      case_eq (nnrc_core_eval h env e); [intros ? eqq1 | intros eqq1];
+      case_eq (nnrc_core_eval h c env e); [intros ? eqq1 | intros eqq1];
       rewrite eqq1 in *;
         simpl in *; try discriminate.
       eapply fun_of_unaryop_normalized; eauto.
     - Case "NNRCLet"%string.
-      simpl; intros.
-      case_eq (nnrc_core_eval h env e1); [intros ? eqq1 | intros eqq1];
+      case_eq (nnrc_core_eval h c env e1); [intros ? eqq1 | intros eqq1];
       rewrite eqq1 in *;
         simpl in *; try discriminate.
-      case_eq (nnrc_core_eval h ((v,d)::env) e2); [intros ? eqq2 | intros eqq2];
+      case_eq (nnrc_core_eval h c ((v,d)::env) e2); [intros ? eqq2 | intros eqq2];
       rewrite eqq2 in *;
         simpl in *; try discriminate.
       inversion H; subst.
       eapply IHe2; eauto.
       constructor; eauto.
     - Case "NNRCFor"%string.
-      simpl; intros.
-      case_eq (nnrc_core_eval h env e1); [intros ? eqq1 | intros eqq1];
+      case_eq (nnrc_core_eval h c env e1); [intros ? eqq1 | intros eqq1];
       rewrite eqq1 in *;
       simpl in *; try discriminate.
       destruct d; try discriminate.
-      specialize (IHe1 _ _ eqq1 H0).
+      specialize (IHe1 _ _ Hc eqq1 H0).
       inversion IHe1; subst.
       apply some_lift in H.
       destruct H; subst.
       constructor.
       apply (rmap_Forall e H2); intros.
-      apply (IHe2 _ _ H).
+      apply (IHe2 _ _ Hc H).
       constructor; eauto.
     - Case "NNRCIf"%string.
-      simpl; intros.
-      case_eq (nnrc_core_eval h env e1); [intros ? eqq1 | intros eqq1];
+      case_eq (nnrc_core_eval h c env e1); [intros ? eqq1 | intros eqq1];
       rewrite eqq1 in *;
       simpl in *; try discriminate.
       destruct d; try discriminate.
       destruct b; eauto.
     - Case "NNRCEither"%string.
-      simpl; intros.
-      case_eq (nnrc_core_eval h env e1); [intros ? eqq1 | intros eqq1];
+      case_eq (nnrc_core_eval h c env e1); [intros ? eqq1 | intros eqq1];
       rewrite eqq1 in *;
       simpl in *; try discriminate.
-      specialize (IHe1 _ _ eqq1 H0).
+      specialize (IHe1 _ _ Hc eqq1 H0).
       destruct d; try discriminate; inversion IHe1; subst.
       + eapply IHe2; eauto.
          constructor; eauto.
@@ -109,7 +106,7 @@ Section cNNRCProp.
       simpl; intros; congruence.
   Qed.
 
-End cNNRCProp.
+End cNNRCNorm.
 
 Hint Resolve nnrc_core_eval_normalized.
 
